
%......................................................................
\subsection{Syntax}\label{sec:syntax}


%......................................................................
\begin{syntaxdiagram}{Program}
  \node[junction,right=of Program] (startl1) {};
  \node[junction,right=of startl1] (bl) {};
  \node[junction,right=of bl] (l) {};
  \node[junction,right=of l] (al) {};
  \node[junction,right=of al] (bcd) {};
  \node[junction,right=of bcd,xshift=3mm] (cd) {};
  \node[junction,right=of cd,xshift=3mm] (acd) {};
  \node[junction,right=of acd] (bvd) {};
  \node[junction,right=of bvd,xshift=7mm] (vd) {};
  \node[junction,right=of vd,xshift=7mm] (avd) {};
  \node[junction,right=of avd] (endl1) {$\cdots$};

  \node[junction,below=of startl1,yshift=-10mm] (startl2) {};
  \node[junction,right=of startl2] (brl) {};
  \node[junction,right=of brl] (rl) {};
  \node[junction,right=of brl] (rl) {};
  \node[junction,right=of rl] (arl) {};
  \node[junction,right=of arl] (bass) {};
  \node[junction,right=of bass,xshift=3mm] (ass) {};
  \node[junction,right=of ass,xshift=3mm] (aass) {};
  \node[junction,right=of aass] (endl2) {$\diamond$};

  \node[nonterminal,below=of l] (Lexicon) {Lexicon};
  \node[nonterminal,below=of cd] (ClassDecls) {ClassDecls};
  \node[nonterminal,below=of vd] (GlobalVarDecls) {GlobalVarDecls};
  \node[nonterminal,below=of rl] (Rules) {Rules};
  \node[nonterminal,below=of ass] (Assertions) {Assertions};
  
\graph [use existing nodes] {
startl1 -- bl -- l -- al -- bcd  -- cd -- acd -- bvd -- vd -- avd -> endl1
};
\graph [use existing nodes] {
startl2 -- brl -- rl -- arl -- bass  -- ass -- aass -> endl2
};

\syndiagAlternative{bl}{Lexicon}{Lexicon}{al}
\syndiagAlternative{bcd}{ClassDecls}{ClassDecls}{acd}
\syndiagAlternative{bvd}{GlobalVarDecls}{GlobalVarDecls}{avd}
\syndiagAlternative{brl}{Rules}{Rules}{arl}
\syndiagAlternative{bass}{Assertions}{Assertions}{aass}
\end{syntaxdiagram}


\begin{syntaxdiagram}{Lexicon}
  \node[junction,right=of Lexicon] (startl1) {};
  \node[terminal,right=of startl1] (lexicon) {\texttt{lexicon}};
  \node[junction,right=of lexicon] (bvar) {};
  \node[terminal,right=of bvar] (var) {\emph{VAR}};
  \node[terminal,right=of var] (arrow) {\texttt{->}};
  \node[terminal,right=of arrow] (string) {\emph{string}};
  \node[junction,right=of string] (astring) {};
  \node[junction,right=of astring] (end) {};
  \node[junction,above=of string] (abs) {};

\graph [use existing nodes] {
startl1 -- lexicon -- bvar -- var -- arrow -- string -- astring -> end
};

\syndiagBridge{astring}{abs}{bvar}
\end{syntaxdiagram}
%......................................................................

%......................................................................
\begin{syntaxdiagram}{ClassDecls}
  \node[junction,right=of ClassDecls] (start) {};
  \node[junction,right=of start,xshift=-3mm] (bdecl) {};
  \node[terminal,right=of bdecl,xshift=-3mm] (class) {\texttt{class}};
  \node[terminal,right=of class,xshift=-3mm] (classname) {\emph{VAR}};
  \node[junction,right=of classname,xshift=-4mm] (bextends) {};
  \node[terminal,right=of bextends,xshift=-4mm] (extends) {\texttt{extends}};
  \node[terminal,right=of extends,xshift=-3mm] (extendsname) {\emph{VAR}};
  \node[junction,right=of extendsname,xshift=-4mm] (bFields) {};
  \node[nonterminal,right=of bFields,xshift=-4mm] (Fields) {Fields};
  \node[junction,right=of Fields,xshift=-3mm] (aFields) {};
  \node[junction,right=of aFields,xshift=-3mm] (end) {};
  \node[junction,above=of extends] (abextends) {};
  \node[junction,below=of extends] (blextends) {};

\graph [use existing nodes] {
start -- bdecl -- class -- classname -- bextends -- extends -- extendsname --
bFields -- Fields -- aFields -> end
};

\syndiagBridge{aFields}{abextends}{bdecl}
\syndiagBridge{bextends}{blextends}{bFields}

\end{syntaxdiagram}
%......................................................................


%......................................................................
\begin{syntaxdiagram}{Fields}
  \node[junction,right=of Fields] (start) {};
  \node[junction,right=of start] (bleftbrace) {};
  \node[terminal,right=of bleftbrace] (leftbrace) {\verb|{|};
  \node[junction,right=of leftbrace] (aleftbrace) {};
  \node[nonterminal,right=of aleftbrace] (VarDecl) {VarDecl};
  \node[junction,right=of VarDecl] (brightbrace) {};
  \node[terminal,right=of brightbrace] (rightbrace) {\verb|}|};
  \node[junction,right=of rightbrace] (arightbrace) {};
  \node[junction,right=of arightbrace] (end) {};
  \node[junction,above=of VarDecl] (abVarDecl) {};
  \node[junction,below=of VarDecl] (blVarDecl) {};
  \node[junction,below=of blVarDecl] (blblVarDecl) {};

\graph [use existing nodes] {
start -- bleftbrace -- leftbrace -- aleftbrace -- VarDecl -- brightbrace --
rightbrace -- arightbrace -> end 
};

\syndiagBridge{brightbrace}{abVarDecl}{aleftbrace}
\syndiagBridge{aleftbrace}{blVarDecl}{brightbrace}
\syndiagBridge{bleftbrace}{blblVarDecl}{arightbrace}
\end{syntaxdiagram}
%......................................................................


%......................................................................
\begin{syntaxdiagram}{GlobalVarDecls}
  \node[junction,right=of GlobalVarDecls] (start) {};
  \node[junction,right=of start] (bdecl) {};
  \node[terminal,right=of bdecl] (decl) {\texttt{decl}};
  \node[nonterminal,right=of decl] (VarDecl) {VarDecl};
  \node[junction,right=of VarDecl] (aVarDecl) {};
  \node[junction,right=of aVarDecl] (end) {};
  \node[junction,above=of VarDecl] (abv) {};

\graph [use existing nodes] {
start -- bdecl -- decl -- VarDecl -- aVarDecl -> end
};

\syndiagBridge{aVarDecl}{abv}{bdecl}
\end{syntaxdiagram}
%......................................................................



%......................................................................
\begin{syntaxdiagram}{VarDecl}
  \node[junction,right=of VarDecl] (start) {};
  \node[junction,right=of start] (bvar) {};
  \node[terminal,right=of bvar] (var) {\emph{VAR}};
  \node[terminal,right=of var] (colon) {\texttt{:}};
  \node[nonterminal,right=of colon] (Tp) {Tp};
  \node[junction,right=of Tp] (aTp) {};
  \node[junction,right=of aTp] (end) {};

\graph [use existing nodes] {
start -- bvar -- var -- colon -- Tp -- aTp -> end
};
\end{syntaxdiagram}
%......................................................................


%......................................................................
\begin{syntaxdiagram}{Rules}
  \node[junction,right=of Rules] (start) {};
  \node[junction,right=of start] (brule) {};
  \node[nonterminal,right=of brule] (Fact) {Fact};
  \node[junction,right=of Fact] (arule) {};
  \node[junction,right=of arule] (end) {};
  \node[junction,above=of Fact] (abfact) {};
  \node[nonterminal,below=of Fact] (Rule) {Rule};

\graph [use existing nodes] {
start -- brule -- Fact -- arule -> end
};

\syndiagBridge{arule}{abfact}{brule}
\syndiagAlternative{brule}{Rule}{Rule}{arule}
\end{syntaxdiagram}
%......................................................................


%......................................................................
\begin{syntaxdiagram}{Rule}
  \node[junction,right=of Rule] (startl1) {};
  \node[terminal,right=of startl1] (rule) {\texttt{rule}};
  \node[terminal,right=of rule] (rname) {\texttt{<} \emph{VAR} \texttt{>}};
  \node[junction,right=of rname,xshift=-4mm] (bfor) {};
  \node[terminal,right=of bfor,xshift=-4mm] (for) {\texttt{for}};
  \node[junction,right=of for,xshift=-3mm] (bVarDecl) {};
  \node[nonterminal,right=of bVarDecl,xshift=-3mm] (VarDecl) {VarDecl};
  \node[junction,right=of VarDecl,xshift=-4mm] (aVarDecl) {};
  \node[junction,right=of aVarDecl,xshift=-4mm] (endl1) {$\cdots$};

  \node[junction,below=of startl1,yshift=-10mm] (start2) {};
  \node[terminal,right=of startl2,xshift=-4mm] (if) {\texttt{if}};
  \node[nonterminal,right=of if,xshift=-3mm] (Expr1) {Expr};
  \node[terminal,right=of Expr1,xshift=-4mm] (then) {\texttt{then}};
  \node[nonterminal,right=of then,xshift=-3mm] (Expr2) {Expr};
  \node[junction,right=of Expr2,xshift=-3mm] (endl2) {};
  \node[junction,above=of VarDecl] (abVarDecl) {};
  \node[terminal,below=of VarDecl] (blVarDecl) {\texttt{,}};

\graph [use existing nodes] {
startl1 -- rule -- rname -- bfor -- for -- bVarDecl -- VarDecl -- aVarDecl -> endl1
};
\graph [use existing nodes] {
startl2 -- if -- Expr1 -- then -- Expr2 -> endl2
};

\syndiagBridge{bfor}{abVarDecl}{aVarDecl}
\syndiagBridge{aVarDecl}{blVarDecl}{bVarDecl}

\end{syntaxdiagram}
%......................................................................


%......................................................................
\begin{syntaxdiagram}{Fact}
  \node[junction,right=of Fact] (startl1) {};
  \node[terminal,right=of startl1] (fact) {\texttt{fact}};
  \node[terminal,right=of fact] (rname) {\texttt{<} \emph{VAR} \texttt{>}};
  \node[junction,right=of rname,xshift=-4mm] (bfor) {};
  \node[terminal,right=of bfor,xshift=-4mm] (for) {\texttt{for}};
  \node[junction,right=of for,xshift=-3mm] (bVarDecl) {};
  \node[nonterminal,right=of bVarDecl,xshift=-3mm] (VarDecl) {VarDecl};
  \node[junction,right=of VarDecl,xshift=-4mm] (aVarDecl) {};
  \node[nonterminal,right=of aVarDecl,xshift=-3mm] (Expr) {Expr};
  \node[junction,right=of Expr,xshift=-4mm] (endl1) {};
  \node[junction,above=of VarDecl] (abVarDecl) {};
  \node[terminal,below=of VarDecl] (blVarDecl) {\texttt{,}};

\graph [use existing nodes] {
startl1 -- fact -- rname -- bfor -- for -- bVarDecl -- VarDecl -- aVarDecl --
Expr -> endl1
};

\syndiagBridge{bfor}{abVarDecl}{aVarDecl}
\syndiagBridge{aVarDecl}{blVarDecl}{bVarDecl}
\end{syntaxdiagram}
%......................................................................


%......................................................................
\begin{syntaxdiagram}{Assertions}
  \node[junction,right=of Assertions] (start) {};
  \node[junction,right=of start] (bassert) {};
  \node[terminal,right=of bassert] (assert) {\texttt{assert}};
  \node[nonterminal,right=of assert] (expr) {Expr};
  \node[junction,right=of expr] (aexpr) {};
  \node[junction,right=of aexpr] (end) {};
  \node[junction,below=of expr] (blexpr) {};
  \node[junction,above=of expr] (abexpr) {};

\graph [use existing nodes] {
start -- bassert -- assert -- expr -- aexpr -> end
};

\syndiagBridge{aexpr}{abexpr}{bassert}
\syndiagBridge{bassert}{blexpr}{aexpr}

\end{syntaxdiagram}
%......................................................................


A \nonterminalref{Program} is the main processing unit. It consists of a
lexicon, a list of class declarations, global variable declarations, rules and
assertions, all of which can be missing.

A \nonterminalref{Lexicon} maps identifiers of the program to GF
strings\remms{Inari: more details}.

Class declarations (\nonterminalref{ClassDecls}) come in several shapes. In
its simplest form, a class declaration introduces a new class and relates it
to a superclass, as in
\begin{lstlisting}
class Lawyer extends Person
\end{lstlisting}  

The \texttt{extends} clause can also be omitted, in which case the superclass
is implicitly assumed to be \texttt{Class} (see \secref{sec:typing} for the
built-in class hierarchy). Thus,
\begin{lstlisting}
class Person
\end{lstlisting}  
is equivalent to:
\begin{lstlisting}
class Person extends Class
\end{lstlisting}

New fields can be added to a class with field declarations
(\nonterminalref{Fields}). These are variable declarations
enclosed in braces; they can also be missing altogether (equivalent to empty
field declarations \texttt{\{\}}). For example, 
\begin{lstlisting}
class Person {
   name : String
   age : Integer }

class Lawyer extends Person {
   companyName : String }
\end{lstlisting}  
introduces two fields \texttt{name} and \texttt{age} to class \texttt{Person},
whereas \texttt{Lawyer} inherits \texttt{name} and \texttt{age} from
\texttt{Person} and in addition defines a third field \texttt{companyName}.

Global variable declarations (\nonterminalref{GlobalVarDecls}) introduce names
that are meant to have global visibility in the program.

In the \nonterminalref{Rules} section, rules and facts can be mixed
arbitrarily. A \nonterminalref{Rule} introduces local variables in a
\texttt{for} clause (which may be omitted if there are no local variables),
followed by a precondition (\texttt{if}) and a postcondition (\texttt{then}),
both assumed to be Boolean expressions. If there are several preconditions,
these have to be conjoined by \emph{and} to form a single formula. 
A \nonterminalref{Fact} is a notational variant of a  \nonterminalref{Rule}
that does not have a precondition (more technically, a fact is mapped to a
rule whose precondition is \texttt{True}).

\nonterminalref{Assertions} are Boolean expressions introduced by the keyword \texttt{assert}.


%......................................................................
\subsection{Typing}\label{sec:typing}



%......................................................................
\subsection{Pragmatics}\label{sec:pragmatics}



%%% Local Variables:
%%% mode: latex
%%% TeX-master: "main"
%%% End:
